dot_wfrel2.v: Build sem_vl_subtype into sem_subtype
Instead of trying to really prove `subtype_to_vl_subtype`, just make it hold by
construction by strengthening sem_subtype.

I did this just after realizing that vl_to_tm is very hard to prove, even with
let in values, because we can't ensure (for arbitrary values) that the closures
close over the same environments (which could be fixable).

Even ignoring that, the proof looks insanely hard because of the complexity of
the necessary inductive hypothesis --- it looks comparable to CPS/ANF conversion.

ecoop17/dot_wfrel2.v
@@ -352,19 +352,20 @@ Definition sem_type (G : tenv) (T : ty) (e: tm) :=
     R_env k env G ->
     etp T k e env.
 
-Definition sem_subtype (G : tenv) (T1 T2: ty) :=
-  wf G T1 /\
-  wf G T2 /\
-  forall k env,
-    R_env k env G ->
-    forall e, etp T1 k e env -> etp T2 k e env.
-
 Definition sem_vl_subtype (G : tenv) (T1 T2: ty) :=
   wf G T1 /\
   wf G T2 /\
   forall k env,
     R_env k env G ->
     forall v, vtp T1 k v env -> vtp T2 k v env.
+
+Definition sem_subtype (G : tenv) (T1 T2: ty) :=
+  wf G T1 /\
+  wf G T2 /\
+  sem_vl_subtype G T1 T2 /\
+  forall k env,
+    R_env k env G ->
+    forall e, etp T1 k e env -> etp T2 k e env.
 
 Hint Unfold wf sem_type sem_subtype sem_vl_subtype etp.
 
@@ -404,6 +405,19 @@ Proof.
       firstorder eauto.
 Qed.
 Hint Resolve vl_subtype_to_subtype.
+
+Lemma subtype_to_vl_subtype : forall G T1 T2,
+    sem_subtype G T1 T2 -> sem_vl_subtype G T1 T2.
+Proof. unfold sem_subtype; tauto. Qed.
+Hint Resolve subtype_to_vl_subtype.
+
+Require Import PropExtensionality.
+Lemma vl_sub_equiv: sem_subtype = sem_vl_subtype.
+Proof.
+  repeat (apply functional_extensionality; intro); apply propositional_extensionality;
+    split; eauto.
+Qed.
+Hint Rewrite vl_sub_equiv.
 
 Lemma and_stp1 : forall env T1 T2 n v, vtp (TAnd T1 T2) n v env -> vtp T1 n v env.
 Proof. intros; vtp_simpl_unfold; tauto. Qed.
@@ -446,23 +460,9 @@ Proof.
   intros; vtp_simpl_unfold; repeat case_match; ev; intros; injectHyps; try contradiction; eauto.
 Qed.
 
-(* Program Definition vl_to_tm (v : vl): { (e, env) : tm * venv | *)
-(*                                         tevalSnmOpt env e (Some v) 0 0 } := *)
-(*   match v with *)
-(*   | vabs env T body => *)
-(*     (tabs T body, env) *)
-(*   | vty env T => *)
-(*     (ttyp T, env) *)
-(*   end. *)
-(* Solve Obligations with program_simplify; unfold tevalSnmOpt in *; intros * Hfuel; destruct n; solve [inverse Hfuel] || reflexivity. *)
-
-(* XXX this isn't true, but we should be able to fix it in a setting with substitution in terms (which depends on substitution in types). *)
 (* Once we define the OFE of semantic types, we can alternatively define a
 language of term realizers that mention no types, not even in ttyp, just like in
 Ahmed's typeless System F. *)
-(* Instead of writing [], just write arbitrary environments right away. *)
-Axiom vl_to_tm: forall (v : vl) , { e : tm | forall env,
-                                 tevalSnmOpt env e (Some v) 0 0 }.
 
 (* We want to relate etp and vtp. *)
 Lemma etp_vtp_j: forall e v k j nm T env,
@@ -506,40 +506,6 @@ Lemma vtp_etp:
     etp T k e env.
 Proof. eauto. Qed.
 Hint Resolve vtp_etp.
-
-Lemma subtype_to_vl_subtype : forall G T1 T2,
-    sem_subtype G T1 T2 -> sem_vl_subtype G T1 T2.
-Proof.
-  (* unfold sem_subtype, sem_vl_subtype; intros; intuition eauto; *)
-  (*   destruct (vl_to_tm v) as [e Heval]; firstorder eauto. *)
-  unfold sem_subtype, sem_vl_subtype; intros * (? & ? & Hsub);
-    split_conj; eauto;
-      intros * Henv * HvT1;
-      destruct (vl_to_tm v) as [e Heval];
-      firstorder eauto.
-  (* specialize (Hsub k env Henv e); *)
-  (*   specialize (Heval env). *)
-  (*   (* assert (wf G T1) by eauto. *) *)
-  (* assert (etp T2 k e env) as [? HeT2]. { *)
-  (*   unfold etp, expr_sem in *; apply Hsub; intuition eauto. *)
-  (*   exists v; unfold tevalSnOpt in *; ev; eval_det; eauto. *)
-  (* } *)
-  (* (* eauto. *) *)
-  (* (* (* unfold etp, expr_sem, tevalSnOpt, tevalSnOpt, tevalSnmOpt in HeT2. *) *) *)
-  (* (* (* eauto. *) *) *)
-  (* (* (* destruct (HeT2 (Some v) 0) as (? & ? & ?); replace (k - 0) with k in * by omega; simpl. eauto. *) *) *)
-Qed.
-
-(* Qed. *)
-Hint Resolve subtype_to_vl_subtype.
-
-Require Import PropExtensionality.
-Lemma vl_sub_equiv: sem_subtype = sem_vl_subtype.
-Proof.
-  repeat (apply functional_extensionality; intro); apply propositional_extensionality;
-    split; eauto.
-Qed.
-Hint Rewrite vl_sub_equiv.
 
 Lemma sem_stp_and : forall G S T1 T2,
     sem_subtype G S T1 ->
@@ -838,11 +804,9 @@ Lemma stp_weak : forall G T1 T2 T,
     sem_subtype G T1 T2 ->
     sem_subtype (T :: G) T1 T2.
 Proof.
-  unfold sem_subtype, wf; simpl; intros * (? & ? & Hsub); split_conj; eauto.
-  intros * Henv * HT1.
-  dependent destruction Henv.
-  (* etp, expr_sem. *)
-  eapply Hsub; eauto.
+  unfold sem_subtype, sem_vl_subtype, wf; simpl; intros * (? & ? & Hvlsub & Hsub); split_conj; eauto; intros * Henv * HT1; dependent destruction Henv.
+  (* eapply Hvlsub; eauto. *)
+  (* eapply Hsub; eauto. *)
 Admitted.
 (*   (* eexists; ev. *) *)
 (*   eauto. *)
